SUCCESS: explicit kinds. Also: bounds on input size

examples/lowparse/LowParse.Spec.Array.fst
@@ -12,17 +12,22 @@ let array_pred (#t: Type) (n: nat) (s: Seq.seq t) : GTot Type0 =
 
 type array (t: Type) (n: nat) = (s: Seq.seq t { array_pred n s } )
 
-let array_type_of_parser_kind_precond
-  (#elem_byte_size: nat)
-  (#k: constant_size_parser_kind)
-  (#b: bool)
-  (#u: unit { strong_parser_kind_consumes_at_least_one_byte (StrongConstantSize (elem_byte_size) k) b } )
-  (#t: Type0)
-  (p: parser (ParserStrong (StrongParserKind (StrongConstantSize elem_byte_size k) b u)) t)
+let array_type_of_parser_kind_precond'
+  (k: parser_kind)
   (array_byte_size: nat)
 : GTot bool
-= elem_byte_size > 0 &&
+= let elem_byte_size = k.parser_kind_low in
+  k.parser_kind_high = Some elem_byte_size &&
+  elem_byte_size > 0 &&
   array_byte_size % elem_byte_size = 0
+
+let array_type_of_parser_kind_precond
+  (#k: parser_kind)
+  (#t: Type0)
+  (p: parser k t)
+  (array_byte_size: nat)
+: GTot bool
+= array_type_of_parser_kind_precond' k array_byte_size
 
 (* TODO: move to FStar.Math.Lemmas *)
 
@@ -38,28 +43,22 @@ let div_nonneg
 
 #reset-options
 
-let array_type_of_parser'
-  (#elem_byte_size: nat)
-  (#k: constant_size_parser_kind)
-  (#b: bool)
-  (#u: unit { strong_parser_kind_consumes_at_least_one_byte (StrongConstantSize (elem_byte_size) k) b } )
+let array_type_of_parser
+  (#k: parser_kind)
   (#t: Type0)
-  (p: parser (ParserStrong (StrongParserKind (StrongConstantSize elem_byte_size k) b u)) t)
+  (p: parser k t)
   (array_byte_size: nat)
 : Pure Type0
   (requires (
     array_type_of_parser_kind_precond p array_byte_size == true
   ))
   (ensures (fun _ -> True))
-= array t (array_byte_size / elem_byte_size)
+= array t (array_byte_size / k.parser_kind_low)
 
 let parse_array_correct
-  (#elem_byte_size: nat)
-  (#k: constant_size_parser_kind)
-  (#b: bool)
-  (#u: unit { strong_parser_kind_consumes_at_least_one_byte (StrongConstantSize (elem_byte_size) k) b } )
+  (#k: parser_kind)
   (#t: Type0)
-  (p: parser (ParserStrong (StrongParserKind (StrongConstantSize elem_byte_size k) b u)) t)
+  (p: parser k t)
   (array_byte_size: nat)
   (u' : unit {array_type_of_parser_kind_precond p array_byte_size == true})
   (b: bytes)
@@ -67,85 +66,27 @@ let parse_array_correct
   (data: Seq.seq t)
 : Lemma
   (requires (parse (parse_flbytes (parse_seq p) array_byte_size) b == Some (data, consumed)))
-  (ensures (array_pred #t (array_byte_size / elem_byte_size) data))
+  (ensures (array_pred #t (array_byte_size / k.parser_kind_low) data))
 = assert (consumed == array_byte_size);
   let b' = Seq.slice b 0 consumed in
   seq_length_constant_size_parser_correct p b';
-  FStar.Math.Lemmas.multiple_division_lemma (Seq.length data) elem_byte_size;
+  FStar.Math.Lemmas.multiple_division_lemma (Seq.length data) k.parser_kind_low;
   ()
 
 let parse_array'
-  (#elem_byte_size: nat)
-  (#k: constant_size_parser_kind)
-  (#b: bool)
-  (#u: unit { strong_parser_kind_consumes_at_least_one_byte (StrongConstantSize (elem_byte_size) k) b } )
+  (#k: parser_kind)
   (#t: Type0)
-  (p: parser (ParserStrong (StrongParserKind (StrongConstantSize elem_byte_size k) b u)) t)
+  (p: parser k t)
   (array_byte_size: nat)
   (precond: unit {array_type_of_parser_kind_precond p array_byte_size == true})
-: Tot (parser (ParserStrong (StrongParserKind (StrongConstantSize array_byte_size ConstantSizeUnknown) (array_byte_size > 0) ())) (array_type_of_parser' p array_byte_size))
-= assert_norm (array_type_of_parser' p array_byte_size == (x: Seq.seq t { array_pred (array_byte_size / elem_byte_size) x}));
-  coerce
-    (parser (ParserStrong (StrongParserKind (StrongConstantSize array_byte_size ConstantSizeUnknown) (array_byte_size > 0) ())) (array_type_of_parser' p array_byte_size))
-    (parse_strengthen (parse_flbytes (parse_seq p) array_byte_size) (array_pred (array_byte_size / elem_byte_size)) (parse_array_correct p array_byte_size precond))
-
-(*
-abstract
-let parse_array_precond
-  (#elem_byte_size: nat)
-  (#k: constant_size_parser_kind)
-  (#b: bool)
-  (#u: unit { strong_parser_kind_consumes_at_least_one_byte (StrongConstantSize (elem_byte_size) k) b } )
-  (#t: Type0)
-  (p: parser (ParserStrong (StrongParserKind (StrongConstantSize elem_byte_size k) b u)) t)
-  (array_byte_size: U32.t)
-: Tot Type0
-= unit -> Lemma
-  (array_type_of_parser_kind_precond p (U32.v array_byte_size))
-
-abstract
-let parse_array_precond_intro
-  (#elem_byte_size: nat)
-  (#k: constant_size_parser_kind)
-  (#b: bool)
-  (#u: unit { strong_parser_kind_consumes_at_least_one_byte (StrongConstantSize (elem_byte_size) k) b } )
-  (#t: Type0)
-  (p: parser (ParserStrong (StrongParserKind (StrongConstantSize elem_byte_size k) b u)) t)
-  (array_byte_size: U32.t)
-  (x: (
-    unit -> Lemma
-    (array_type_of_parser_kind_precond p (U32.v array_byte_size))
-  ))
-: Tot (parse_array_precond p array_byte_size)
-= x
-
-abstract
-let parse_array_precond_elim
-  (#elem_byte_size: nat)
-  (#k: constant_size_parser_kind)
-  (#b: bool)
-  (#u: unit { strong_parser_kind_consumes_at_least_one_byte (StrongConstantSize (elem_byte_size) k) b } )
-  (#t: Type0)
-  (#p: parser (ParserStrong (StrongParserKind (StrongConstantSize elem_byte_size k) b u)) t)
-  (#array_byte_size: U32.t)
-  (x: parse_array_precond p array_byte_size)
-: Lemma
-  (array_type_of_parser_kind_precond p (U32.v array_byte_size))
-= x ()
-
-let array_type_of_parser
-  (#elem_byte_size: nat)
-  (#k: constant_size_parser_kind)
-  (#b: bool)
-  (#u: unit { strong_parser_kind_consumes_at_least_one_byte (StrongConstantSize (elem_byte_size) k) b } )
-  (#t: Type0)
-  (#p: parser (ParserStrong (StrongParserKind (StrongConstantSize elem_byte_size k) b u)) t)
-  (#array_byte_size: U32.t)
-  (precond: parse_array_precond p array_byte_size)
-: Tot Type0
-= parse_array_precond_elim precond;
-  array_type_of_parser' p (U32.v array_byte_size)
-*)
+: Tot (parser (parse_flbytes_kind array_byte_size) (array_type_of_parser p array_byte_size))
+= let p' : parser (parse_flbytes_kind array_byte_size) (Seq.seq t) =
+    (parse_flbytes (parse_seq p) array_byte_size)
+  in
+  assert_norm (array_type_of_parser p array_byte_size == (x: Seq.seq t { array_pred (array_byte_size / k.parser_kind_low) x}));
+  coerce_parser
+    (array_type_of_parser p array_byte_size)
+    (parse_strengthen p' (array_pred (array_byte_size / k.parser_kind_low)) (parse_array_correct p array_byte_size precond))
 
 let mod_plus_p_r
   (a: nat)
@@ -162,17 +103,18 @@ let mod_plus_p_l
 = mod_plus_p_r a p
 
 val parse_total_constant_size_elem_parse_list_total
-  (#elem_byte_size: nat)
-  (#b: bool)
-  (#u: unit { strong_parser_kind_consumes_at_least_one_byte (StrongConstantSize (elem_byte_size) ConstantSizeTotal) b } )
+  (#k: parser_kind)
   (#t: Type0)
-  (p: parser (ParserStrong (StrongParserKind (StrongConstantSize elem_byte_size ConstantSizeTotal) b u)) t)
+  (p: parser k t)
   (b: bytes)
 : Lemma
   (requires (
+    k.parser_kind_high == Some k.parser_kind_low /\
+    k.parser_kind_total == true /\ (
+    let elem_byte_size = k.parser_kind_low in
     elem_byte_size > 0 /\
     Seq.length b % elem_byte_size == 0
-  ))
+  )))
   (ensures (
     Some? (parse (PL.parse_list p) b)
   ))
@@ -180,9 +122,10 @@ val parse_total_constant_size_elem_parse_list_total
 
 // #reset-options "--z3rlimit 128 --max_fuel 8 --max_ifuel 8 --z3cliopt smt.arith.nl=false"
 
-#set-options "--z3rlimit 16"
+#set-options "--z3rlimit 32"
 
-let rec parse_total_constant_size_elem_parse_list_total #elem_byte_size #b #u #t p b =
+let rec parse_total_constant_size_elem_parse_list_total #k #t p b =
+  let elem_byte_size : pos = k.parser_kind_low in
   if Seq.length b = 0
   then ()
   else begin
@@ -191,6 +134,7 @@ let rec parse_total_constant_size_elem_parse_list_total #elem_byte_size #b #u #t
     let pe = parse p b in
     assert (Some? pe);
     let (Some (_, consumed)) = pe in
+    is_constant_size_parser_equiv elem_byte_size p;
     assert ((consumed <: nat) == elem_byte_size);
     let b' = Seq.slice b consumed (Seq.length b) in
     assert (Seq.length b' == Seq.length b - consumed);
@@ -204,13 +148,14 @@ let rec parse_total_constant_size_elem_parse_list_total #elem_byte_size #b #u #t
 #reset-options
 
 val parse_total_constant_size_elem_parse_array_total'
-  (#elem_byte_size: nat)
-  (#b: bool)
-  (#u: unit { strong_parser_kind_consumes_at_least_one_byte (StrongConstantSize (elem_byte_size) ConstantSizeTotal) b } )
+  (#k: parser_kind)
   (#t: Type0)
-  (p: parser (ParserStrong (StrongParserKind (StrongConstantSize elem_byte_size ConstantSizeTotal) b u)) t)
+  (p: parser k t)
   (array_byte_size: nat)
-  (precond: unit {array_type_of_parser_kind_precond p array_byte_size == true})
+  (precond: unit {
+    k.parser_kind_total == true /\
+    array_type_of_parser_kind_precond p array_byte_size == true
+  })
   (b: bytes)
 : Lemma
   (requires (
@@ -222,7 +167,7 @@ val parse_total_constant_size_elem_parse_array_total'
 
 #set-options "--z3rlimit 16"
 
-let parse_total_constant_size_elem_parse_array_total' #elem_byte_size #b #u #t p array_byte_size precond b =
+let parse_total_constant_size_elem_parse_array_total' #k #t p array_byte_size precond b =
   let b' = Seq.slice b 0 array_byte_size in
   parse_total_constant_size_elem_parse_list_total p b';
   parse_seq_correct p b'
@@ -230,50 +175,53 @@ let parse_total_constant_size_elem_parse_array_total' #elem_byte_size #b #u #t p
 #reset-options
 
 let parse_total_constant_size_elem_parse_array_total
-  (#elem_byte_size: nat)
-  (#k: constant_size_parser_kind)
-  (#b: bool)
-  (#u: unit { strong_parser_kind_consumes_at_least_one_byte (StrongConstantSize (elem_byte_size) k) b } )
+  (#k: parser_kind)
   (#t: Type0)
-  (p: parser (ParserStrong (StrongParserKind (StrongConstantSize elem_byte_size k) b u)) t)
+  (p: parser k t)
   (array_byte_size: nat)
   (precond: unit {array_type_of_parser_kind_precond p array_byte_size == true})
 : Lemma
   (ensures (
-    ConstantSizeTotal? k ==>
+    k.parser_kind_total == true ==>
     is_total_constant_size_parser array_byte_size (parse_array' p array_byte_size precond)
   ))
-= if ConstantSizeTotal? k
+= if k.parser_kind_total
   then
-    let p' : parser (ParserStrong (StrongParserKind (StrongConstantSize elem_byte_size ConstantSizeTotal) b u)) t = p in
-    Classical.forall_intro (Classical.move_requires (parse_total_constant_size_elem_parse_array_total' p' array_byte_size ()))
+    Classical.forall_intro (Classical.move_requires (parse_total_constant_size_elem_parse_array_total' p array_byte_size ()))
   else ()
 
+let parse_array_kind
+  (k: parser_kind)
+  (array_byte_size: nat)
+: Pure parser_kind
+  (requires (array_type_of_parser_kind_precond' k array_byte_size))
+  (ensures (fun _ -> True))
+= {
+    parser_kind_low = array_byte_size;
+    parser_kind_high = Some array_byte_size;
+    parser_kind_total = k.parser_kind_total;
+    parser_kind_subkind = Some ParserStrong;
+  }
+
 let parse_array_prop
-  (#elem_byte_size: nat)
-  (#k: constant_size_parser_kind)
-  (#b: bool)
-  (#u: unit { strong_parser_kind_consumes_at_least_one_byte (StrongConstantSize (elem_byte_size) k) b } )
+  (#k: parser_kind)
   (#t: Type0)
-  (p: parser (ParserStrong (StrongParserKind (StrongConstantSize elem_byte_size k) b u)) t)
+  (p: parser k t)
   (array_byte_size: nat)
   (precond: unit { array_type_of_parser_kind_precond p array_byte_size } )
 : Lemma
-  (parser_kind_prop (ParserStrong (StrongParserKind (StrongConstantSize (array_byte_size) k) (array_byte_size > 0) ())) (parse_array' p (array_byte_size) precond))
+  (parser_kind_prop (parse_array_kind k array_byte_size) (parse_array' p (array_byte_size) precond))
 = parse_total_constant_size_elem_parse_array_total p array_byte_size precond
 
 let parse_array
-  (#elem_byte_size: nat)
-  (#k: constant_size_parser_kind)
-  (#b: bool)
-  (#u: unit { strong_parser_kind_consumes_at_least_one_byte (StrongConstantSize (elem_byte_size) k) b } )
+  (#k: parser_kind)
   (#t: Type0)
-  (p: parser (ParserStrong (StrongParserKind (StrongConstantSize elem_byte_size k) b u)) t)
-  (array_byte_size: U32.t)
-  (precond: unit { array_type_of_parser_kind_precond p (U32.v array_byte_size) == true } )
-: Tot (parser (ParserStrong (StrongParserKind (StrongConstantSize (U32.v array_byte_size) k) (U32.v array_byte_size > 0) ())) (array_type_of_parser' p (U32.v array_byte_size)))
-= parse_array_prop p (U32.v array_byte_size) precond ;
-  strengthen (ParserStrong (StrongParserKind (StrongConstantSize (U32.v array_byte_size) k) (U32.v array_byte_size > 0) ())) (parse_array' p (U32.v array_byte_size) precond)
+  (p: parser k t)
+  (array_byte_size: nat)
+  (precond: unit { array_type_of_parser_kind_precond p array_byte_size == true } )
+: Tot (parser (parse_array_kind k array_byte_size) (array_type_of_parser p array_byte_size))
+= parse_array_prop p (array_byte_size) precond ;
+  strengthen (parse_array_kind k array_byte_size) (parse_array' p array_byte_size precond)
 
 
 include LowParse.Spec.VLBytes
@@ -285,56 +233,44 @@ let vlarray_pred (#t: Type) (min max: nat) (s: Seq.seq t) : GTot Type0 =
 type vlarray (t: Type) (min max: nat) =
   (s: Seq.seq t {vlarray_pred min max s})
 
-let vlarray_type_of_parser_kind_precond'
-  (#elem_byte_size: nat)
-  (#k: constant_size_parser_kind)
-  (#b: bool)
-  (#u: unit { strong_parser_kind_consumes_at_least_one_byte (StrongConstantSize (elem_byte_size) k) b } )
-  (#t: Type0)
-  (p: parser (ParserStrong (StrongParserKind (StrongConstantSize elem_byte_size k) b u)) t)
-  (array_byte_size_min array_byte_size_max: nat) : GTot bool =
-  elem_byte_size > 0 &&
-  array_byte_size_min % elem_byte_size = 0 &&
-  array_byte_size_max % elem_byte_size = 0 &&
-  array_byte_size_max > 0
-
 let vlarray_type_of_parser_kind_precond
-  (#elem_byte_size: nat)
-  (#k: constant_size_parser_kind)
-  (#b: bool)
-  (#u: unit { strong_parser_kind_consumes_at_least_one_byte (StrongConstantSize (elem_byte_size) k) b } )
+  (#k: parser_kind)
   (#t: Type0)
-  (p: parser (ParserStrong (StrongParserKind (StrongConstantSize elem_byte_size k) b u)) t)
-  (array_byte_size_min array_byte_size_max: U32.t) : GTot bool =
-  vlarray_type_of_parser_kind_precond' p (U32.v array_byte_size_min) (U32.v array_byte_size_max)
+  (p: parser k t)
+  (array_byte_size_min array_byte_size_max: nat)
+: GTot bool
+= k.parser_kind_high = Some k.parser_kind_low && (
+    let elem_byte_size = k.parser_kind_low in
+    elem_byte_size > 0 &&
+    array_byte_size_min % elem_byte_size = 0 &&
+    array_byte_size_max % elem_byte_size = 0 &&
+    array_byte_size_min <= array_byte_size_max &&
+    array_byte_size_max > 0 &&
+    array_byte_size_max < 4294967296
+  )
 
-val vlarray_type_of_parser'
-  (#elem_byte_size: nat)
-  (#k: constant_size_parser_kind)
-  (#b: bool)
-  (#u: unit { strong_parser_kind_consumes_at_least_one_byte (StrongConstantSize (elem_byte_size) k) b } )
+val vlarray_type_of_parser
+  (#k: parser_kind)
   (#t: Type0)
-  (p: parser (ParserStrong (StrongParserKind (StrongConstantSize elem_byte_size k) b u)) t)
-  (array_byte_size_min array_byte_size_max: U32.t)
+  (p: parser k t)
+  (array_byte_size_min array_byte_size_max: nat)
 : Pure Type0
   (requires (
-    vlarray_type_of_parser_kind_precond #elem_byte_size #k #b #u #t p array_byte_size_min array_byte_size_max
+    vlarray_type_of_parser_kind_precond p array_byte_size_min array_byte_size_max
   ))
   (ensures (fun _ -> True))
   
-let vlarray_type_of_parser' #elem_byte_size #k #b #u #t p array_byte_size_min array_byte_size_max =
-  let min : nat = U32.v array_byte_size_min / elem_byte_size in
-  let max : nat = U32.v array_byte_size_max / elem_byte_size in
+let vlarray_type_of_parser #k #t p array_byte_size_min array_byte_size_max =
+  let elem_byte_size : pos = k.parser_kind_low in
+  let min : nat = array_byte_size_min / elem_byte_size in
+  let max : nat = array_byte_size_max / elem_byte_size in
   vlarray t min max
 
 val parse_vlarray_correct
-  (#elem_byte_size: nat)
-  (#k: constant_size_parser_kind)
-  (#b: bool)
-  (#u: unit { strong_parser_kind_consumes_at_least_one_byte (StrongConstantSize (elem_byte_size) k) b } )
+  (#k: parser_kind)
   (#t: Type0)
-  (p: parser (ParserStrong (StrongParserKind (StrongConstantSize elem_byte_size k) b u)) t)
-  (array_byte_size_min array_byte_size_max: U32.t)
+  (p: parser k t)
+  (array_byte_size_min array_byte_size_max: nat)
   (u: unit { vlarray_type_of_parser_kind_precond p array_byte_size_min array_byte_size_max == true })
   (b: bytes)
   (consumed: consumed_length b)
@@ -344,12 +280,14 @@ val parse_vlarray_correct
     parse (parse_bounded_vlbytes array_byte_size_min array_byte_size_max (parse_seq p)) b == Some (data, consumed)
   ))
   (ensures (
-    vlarray_pred (U32.v array_byte_size_min / elem_byte_size) (U32.v array_byte_size_max / elem_byte_size) data
+    let elem_byte_size : pos = k.parser_kind_low in
+    vlarray_pred (array_byte_size_min / elem_byte_size) (array_byte_size_max / elem_byte_size) data
   ))
 
 // #set-options "--z3rlimit 1024"
 
-let parse_vlarray_correct #elem_byte_size #k #b #u #t p array_byte_size_min array_byte_size_max u b consumed data =
+let parse_vlarray_correct #k #t p array_byte_size_min array_byte_size_max u b consumed data =
+  let elem_byte_size : pos = k.parser_kind_low in
 (*
   let sz : integer_size = log256 array_byte_size_max in
   assume (consumed >= sz);
@@ -363,90 +301,19 @@ let parse_vlarray_correct #elem_byte_size #k #b #u #t p array_byte_size_min arra
   FStar.Math.Lemmas.lemma_div_le (U32.v array_byte_size_min) consumed' elem_byte_size ;
   FStar.Math.Lemmas.lemma_div_le consumed' (U32.v array_byte_size_max) elem_byte_size
 *)
-  assume (vlarray_pred (U32.v array_byte_size_min / elem_byte_size) (U32.v array_byte_size_max / elem_byte_size) data)
+  assume (vlarray_pred (array_byte_size_min / elem_byte_size) (array_byte_size_max / elem_byte_size) data)
 
 #reset-options
 
-let parse_vlarray'
-  (#elem_byte_size: nat)
-  (#k: constant_size_parser_kind)
-  (#b: bool)
-  (#u: unit { strong_parser_kind_consumes_at_least_one_byte (StrongConstantSize (elem_byte_size) k) b } )
-  (#t: Type0)
-  (p: parser (ParserStrong (StrongParserKind (StrongConstantSize elem_byte_size k) b u)) t)
-  (array_byte_size_min array_byte_size_max: U32.t)
-  (precond: unit {vlarray_type_of_parser_kind_precond p array_byte_size_min array_byte_size_max == true})
-: Tot (parser (ParserStrong (StrongParserKind StrongUnknown true ())) (vlarray_type_of_parser' p array_byte_size_min array_byte_size_max))
-= parse_strengthen
-    (parse_bounded_vlbytes array_byte_size_min array_byte_size_max (parse_seq p))
-    (vlarray_pred (U32.v array_byte_size_min / elem_byte_size) (U32.v array_byte_size_max / elem_byte_size))
-    (parse_vlarray_correct p array_byte_size_min array_byte_size_max precond)
-
-(*
-abstract
-let parse_vlarray_precond
-  (#elem_byte_size: nat)
-  (#k: constant_size_parser_kind)
-  (#b: bool)
-  (#u: unit { strong_parser_kind_consumes_at_least_one_byte (StrongConstantSize (elem_byte_size) k) b } )
-  (#t: Type0)
-  (p: parser (ParserStrong (StrongParserKind (StrongConstantSize elem_byte_size k) b u)) t)
-  (array_byte_size_min array_byte_size_max: U32.t)
-: Tot Type0
-= unit -> Lemma
-  (vlarray_type_of_parser_kind_precond p array_byte_size_min array_byte_size_max)
-
-abstract
-let parse_vlarray_precond_intro
-  (#elem_byte_size: nat)
-  (#k: constant_size_parser_kind)
-  (#b: bool)
-  (#u: unit { strong_parser_kind_consumes_at_least_one_byte (StrongConstantSize (elem_byte_size) k) b } )
-  (#t: Type0)
-  (p: parser (ParserStrong (StrongParserKind (StrongConstantSize elem_byte_size k) b u)) t)
-  (array_byte_size_min array_byte_size_max: U32.t)
-  (x: (unit -> Lemma
-    (vlarray_type_of_parser_kind_precond p array_byte_size_min array_byte_size_max)
-  ))
-: Tot (parse_vlarray_precond p array_byte_size_min array_byte_size_max)
-= x
-
-abstract
-let parse_vlarray_precond_elim
-  (#elem_byte_size: nat)
-  (#k: constant_size_parser_kind)
-  (#b: bool)
-  (#u: unit { strong_parser_kind_consumes_at_least_one_byte (StrongConstantSize (elem_byte_size) k) b } )
-  (#t: Type0)
-  (#p: parser (ParserStrong (StrongParserKind (StrongConstantSize elem_byte_size k) b u)) t)
-  (#array_byte_size_min #array_byte_size_max: U32.t)
-  (x: parse_vlarray_precond p array_byte_size_min array_byte_size_max)
-: Lemma
-  (vlarray_type_of_parser_kind_precond p array_byte_size_min array_byte_size_max)
-= x ()
-
-let vlarray_type_of_parser
-  (#elem_byte_size: nat)
-  (#k: constant_size_parser_kind)
-  (#b: bool)
-  (#u: unit { strong_parser_kind_consumes_at_least_one_byte (StrongConstantSize (elem_byte_size) k) b } )
-  (#t: Type0)
-  (#p: parser (ParserStrong (StrongParserKind (StrongConstantSize elem_byte_size k) b u)) t)
-  (#array_byte_size_min #array_byte_size_max: U32.t)
-  (precond: parse_vlarray_precond p array_byte_size_min array_byte_size_max)
-: Tot Type0
-= parse_vlarray_precond_elim precond;
-  vlarray_type_of_parser' p array_byte_size_min array_byte_size_max
-
 let parse_vlarray
-  (#elem_byte_size: nat)
-  (#k: constant_size_parser_kind)
-  (#b: bool)
-  (#u: unit { strong_parser_kind_consumes_at_least_one_byte (StrongConstantSize (elem_byte_size) k) b } )
+  (#k: parser_kind)
   (#t: Type0)
-  (#p: parser (ParserStrong (StrongParserKind (StrongConstantSize elem_byte_size k) b u)) t)
-  (#array_byte_size_min #array_byte_size_max: U32.t)
-  (precond: parse_vlarray_precond p array_byte_size_min array_byte_size_max)
-: Tot (parser (ParserStrong (StrongParserKind StrongUnknown true ())) (vlarray_type_of_parser precond))
-= parse_vlarray_precond_elim precond;
-  parse_vlarray' p array_byte_size_min array_byte_size_max ()
+  (p: parser k t)
+  (array_byte_size_min array_byte_size_max: nat)
+  (precond: unit {vlarray_type_of_parser_kind_precond p array_byte_size_min array_byte_size_max == true})
+: Tot (parser (parse_bounded_vlbytes_kind array_byte_size_min array_byte_size_max) (vlarray_type_of_parser p array_byte_size_min array_byte_size_max))
+= let elem_byte_size : pos = k.parser_kind_low in
+  parse_strengthen
+    (parse_bounded_vlbytes array_byte_size_min array_byte_size_max (parse_seq p))
+    (vlarray_pred (array_byte_size_min / elem_byte_size) (array_byte_size_max / elem_byte_size))
+    (parse_vlarray_correct p array_byte_size_min array_byte_size_max precond)
